include predicate mask in state, some restructuring

TotalSemantics.thy
@@ -1,188 +1,10 @@
 theory TotalSemantics
-imports Viper.ViperLang TotalExpressions "HOL-Eisbach.Eisbach" "HOL-Eisbach.Eisbach_Tools"
+imports Viper.ViperLang TotalExpressions "HOL-Eisbach.Eisbach" "HOL-Eisbach.Eisbach_Tools" TotalUtil
 begin
 
 (*datatype 'a result = Failure | Set (select_set: "'a full_total_state set")*)
-
 datatype 'a standard_result = RMagic | RFailure | RNormal "'a full_total_state"
 
-fun update_store_total :: "'a full_total_state \<Rightarrow> var \<Rightarrow> 'a val \<Rightarrow> 'a full_total_state"
-  where "update_store_total \<omega> x v = ((get_store_total \<omega>)(x \<mapsto> v), get_trace_total \<omega>, get_hm_total_full \<omega>)"
-
-lemma update_store_total_trace_same: "get_trace_total (update_store_total \<omega> x v) = get_trace_total \<omega>"
-  by simp
-
-lemma update_store_total_hm_same: "get_hm_total_full (update_store_total \<omega> x v) = get_hm_total_full \<omega>"
-  by simp
-
-lemma update_store_total_heap_same: "get_heap_total_full (update_store_total \<omega> x v) = get_heap_total_full \<omega>"
-  by simp
-
-lemma update_store_total_mask_same: "get_mask_total_full (update_store_total \<omega> x v) = get_mask_total_full \<omega>"
-  by simp
-
-fun update_trace_total :: "'a full_total_state \<Rightarrow> 'a total_trace \<Rightarrow> 'a full_total_state"
-  where "update_trace_total \<omega> \<pi> = (get_store_total \<omega>, \<pi>, get_hm_total_full \<omega>)"
-
-lemma update_trace_total_store_same: "get_store_total (update_trace_total \<omega> \<pi>) = get_store_total \<omega>"
-  by simp
-
-lemma update_trace_total_hm_same: "get_hm_total_full (update_trace_total \<omega> \<pi>) = get_hm_total_full \<omega>"
-  by simp
-
-lemma update_trace_total_heap_same: "get_heap_total_full (update_trace_total \<omega> \<pi>) = get_heap_total_full \<omega>"
-  by simp
-
-lemma update_trace_total_mask_same: "get_mask_total_full (update_trace_total \<omega> \<pi>) = get_mask_total_full \<omega>"
-  by simp
-
-definition update_heap_total :: "'a total_state \<Rightarrow> heap_loc \<Rightarrow> 'a val \<Rightarrow> 'a total_state"
-  where "update_heap_total mh l v = Abs_total_state ((get_mask_total mh), (get_heap_total mh)(l := v))"
-
-definition update_mask_total :: "'a total_state \<Rightarrow> mask \<Rightarrow> 'a total_state"
-  where "update_mask_total mh m' = Abs_total_state (m', get_heap_total mh)"
-
-lemma Abs_total_state_inverse_2:
-  assumes "wf_pre_total_state (m,h)"
-  shows "Rep_total_state (Abs_total_state (m,h)) = (m,h)"
-  using assms Abs_total_state_inverse
-  by blast
-
-lemma get_update_mask_total: 
-  assumes "wf_mask_simple m0"
-  shows   "get_mask_total (update_mask_total mh m0) = m0"
-  unfolding update_mask_total_def
-  using assms
-  by (simp add: Abs_total_state_inverse_2)
-
-lemma update_mask_total_multiple: 
-  assumes "wf_mask_simple m0" and "wf_mask_simple m2"
-  shows   "update_mask_total (update_mask_total mh m0) m1 = update_mask_total mh m1"
-  unfolding update_mask_total_def  
-  using assms
-  by (simp add: Abs_total_state_inverse_2)
-
-lemma update_heap_total_mask_same: "get_mask_total (update_heap_total \<phi> l v) = get_mask_total \<phi>"
-  unfolding update_heap_total_def
-  by (metis Abs_total_state_inverse_2 fst_conv get_mask_total.simps get_mask_total_wf wf_pre_total_state.simps)
-
-lemma Rep_total_state_inj: "Rep_total_state a = Rep_total_state b \<Longrightarrow> a = b"
-  by (metis Rep_total_state_inverse)
-
-lemma update_heap_total_overwrite: "update_heap_total (update_heap_total mh l v1) l v2 = update_heap_total mh l v2"
-  apply (rule total_state_eq)
-   apply (simp only: update_heap_total_mask_same)
-  by (metis Abs_total_state_inverse_2 fun_upd_upd get_heap_total.simps get_mask_total_wf snd_conv update_heap_total_def wf_pre_total_state.simps)
-
-lemma update_heap_total_lookup_1: "get_heap_total (update_heap_total \<phi> l v) l = v"
-  by (metis (no_types, lifting) Abs_total_state_inverse_2 fun_upd_eqD fun_upd_triv get_heap_total.simps get_mask_total_wf snd_conv update_heap_total_def wf_pre_total_state.simps)
-
-lemma update_heap_total_lookup_2: "l1 \<noteq> l2 \<Longrightarrow> get_heap_total (update_heap_total \<phi> l1 v) l2 = get_heap_total \<phi> l2"
-  by (metis (no_types, lifting) Abs_total_state_inverse_2 fun_upd_idem_iff fun_upd_triv fun_upd_twist get_heap_total.elims get_mask_total_wf sndI update_heap_total_def wf_pre_total_state.simps)
-
-fun update_heap_total_full :: "'a full_total_state \<Rightarrow> heap_loc \<Rightarrow> 'a val \<Rightarrow> 'a full_total_state"
-  where "update_heap_total_full \<omega> l v = (get_store_total \<omega>, get_trace_total \<omega>, update_heap_total (get_hm_total_full \<omega>) l v )"
-
-lemma update_heap_total_full_lookup_1: "get_heap_total_full (update_heap_total_full \<phi> l v) l = v"
-  by (metis get_heap_total_full.simps get_hm_total_full.simps snd_conv update_heap_total_full.simps update_heap_total_lookup_1)
-
-lemma update_heap_total_full_lookup_2: "l1 \<noteq> l2 \<Longrightarrow> get_heap_total_full (update_heap_total_full \<phi> l1 v) l2 = get_heap_total_full \<phi> l2"
-  by (metis get_heap_total_full.simps get_hm_total_full.simps snd_conv update_heap_total_full.simps update_heap_total_lookup_2)
-
-lemma update_heap_total_overwrite_full: "update_heap_total_full (update_heap_total_full \<omega> l v1) l v2 = update_heap_total_full \<omega> l v2"
-  apply (rule full_total_state_eq)
-     apply simp
-    apply simp
-   apply (simp add: update_heap_total_overwrite)
-  by (metis get_hm_total_full.elims get_mask_total_full.elims snd_conv update_heap_total_full.simps update_heap_total_mask_same)
-  
-fun update_mask_total_full :: "'a full_total_state \<Rightarrow> mask \<Rightarrow> 'a full_total_state"
-  where "update_mask_total_full \<omega> m = (get_store_total \<omega>, get_trace_total \<omega>, update_mask_total (get_hm_total_full \<omega>) m)"
-
-lemma update_heap_total_full_mask_same: "get_mask_total_full (update_heap_total_full \<omega> l v) = get_mask_total_full \<omega>"
-  by (metis get_hm_total_full.simps get_mask_total_full.simps snd_conv update_heap_total_full.simps update_heap_total_mask_same)
-
-lemma get_update_mask_total_full: 
-  assumes "wf_mask_simple m0"
-  shows   "get_mask_total_full (update_mask_total_full mh m0) = m0"
-  using assms get_update_mask_total
-  by auto
-
-lemma update_mask_total_full_same:
-  "(update_mask_total_full \<omega> (get_mask_total_full \<omega>)) = \<omega>"
-  by (simp add: update_mask_total_def Rep_total_state_inverse)
-
-lemma update_mask_total_same_heap: 
-  assumes "wf_mask_simple m"
-  shows "get_heap_total (update_mask_total \<phi> m) = get_heap_total \<phi>"
-  unfolding update_mask_total_def
-  using assms
-  by (simp add: Abs_total_state_inverse)
-
-lemma update_mask_total_full_same_heap: 
-  assumes "wf_mask_simple m"
-  shows "get_heap_total_full (update_mask_total_full \<phi> m) = get_heap_total_full \<phi>"
-  using assms update_mask_total_same_heap
-  by auto
-  
-lemma update_mask_total_full_multiple: 
-  assumes "wf_mask_simple m0"
-  shows   "update_mask_total_full (update_mask_total_full \<omega> m0) m1 = update_mask_total_full \<omega> m1"
-  using assms
-  using update_mask_total_multiple by fastforce  
-
-definition singleton_total_pred :: "heap_loc \<Rightarrow> (prat \<Rightarrow> 'a val \<Rightarrow> bool) \<Rightarrow> 'a store \<Rightarrow> 'a total_trace \<Rightarrow> ('a full_total_state) set"
-  where "singleton_total_pred l P \<sigma> \<tau> = { (\<sigma>, \<tau>, Abs_total_state (m,h)) |m h. P (m l) (h l)}"
-
-(*
-lemma singleton_total_pred_sat: 
-  assumes "\<omega> \<in> singleton_total_pred l P \<sigma> \<tau>"
-  shows "P ( (get_mask_total_full \<omega>) l) ((get_heap_total_full \<omega>) l)"
-proof -
-  obtain \<sigma> \<tau> \<phi> where "\<omega> = (\<sigma>,\<tau>,\<phi>)"
-    using prod_cases3 by blast
-  with assms have "P ((get_mask_total \<phi>) l) ((get_heap_total \<phi>) l)"
-    
-  from assms 
-  have 
-  show ?thesis
-    apply simp
-    apply clarify
-*)
-
-(*
-definition singleton_total :: "bool \<Rightarrow> heap_loc \<Rightarrow> prat \<Rightarrow> 'a val \<Rightarrow> 'a store \<Rightarrow> 'a total_trace \<Rightarrow> ('a full_total_state) set"
-  where "singleton_total havoc_new l p v \<sigma> \<tau> = singleton_total_pred l (\<lambda> p' v'. p = p' \<and> (\<not>havoc_new \<longrightarrow> v = v')) \<sigma> \<tau>"
-*)
-
-definition singleton_total :: "bool \<Rightarrow> heap_loc \<Rightarrow> prat \<Rightarrow> 'a val \<Rightarrow> 'a store \<Rightarrow> 'a total_trace \<Rightarrow> ('a full_total_state) set"
-  where "singleton_total havoc_new l p v \<sigma> \<tau> = 
-           { \<omega> | \<omega>. get_store_total \<omega> = \<sigma> \<and> get_trace_total \<omega> = \<tau> \<and> 
-                    get_mask_total_full \<omega> = (zero_mask(l := p)) \<and> (\<not>havoc_new \<longrightarrow> get_heap_total_full \<omega> l = v)}"
-
-definition singleton_total_wildcard :: "bool \<Rightarrow> heap_loc \<Rightarrow> 'a val \<Rightarrow> 'a store \<Rightarrow> 'a total_trace \<Rightarrow> ('a full_total_state) set"
-  where "singleton_total_wildcard havoc_new l v \<sigma> \<tau> =
-           { \<omega> | \<omega> p. p \<noteq> pnone \<and> get_store_total \<omega> = \<sigma> \<and> get_trace_total \<omega> = \<tau> \<and> 
-                    get_mask_total_full \<omega> = (zero_mask(l := p)) \<and> (\<not>havoc_new \<longrightarrow> get_heap_total_full \<omega> l = v)}"
-
-definition singleton_total_only_mask :: "heap_loc \<Rightarrow> prat \<Rightarrow> 'a store \<Rightarrow> 'a total_trace \<Rightarrow> ('a full_total_state) set"
-  where "singleton_total_only_mask l p \<sigma> \<tau> = singleton_total_pred l (\<lambda> p' v'. p = p') \<sigma> \<tau>"
-
-fun map_result_2 :: "(mask \<Rightarrow> (mask set) option) \<Rightarrow> (mask set) option \<Rightarrow> (mask set) option"
-  where 
-    "map_result_2 f None = None"
-  | "map_result_2 f (Some xs) = (if \<exists>x \<in> xs. f x = None then None else Some (\<Union>x \<in> xs. the (f x))) "
-
-
-fun get_address_opt :: "'a val \<Rightarrow> address option"
-  where 
-    "get_address_opt (VRef (Address a)) = Some a"
-  | "get_address_opt _ = None"
-
-fun option_fold :: "('a \<Rightarrow> 'b) \<Rightarrow> 'b \<Rightarrow> 'a option \<Rightarrow> 'b"
-  where 
-    "option_fold f e (Some x) = f x"
-  | "option_fold f e None = e"
 
 definition inhale_perm_single :: "bool \<Rightarrow>'a full_total_state \<Rightarrow> heap_loc \<Rightarrow> prat option \<Rightarrow> 'a full_total_state set"
   where "inhale_perm_single havoc_new \<omega> l p_opt =
@@ -214,7 +36,7 @@ inductive red_inhale :: "program \<Rightarrow> 'a interp \<Rightarrow> bool \<Ri
   (** if-else **)
  | InhImpTrue: 
    "\<lbrakk> wd_pure_exp_total Pr \<Delta> CInhale e \<omega>; 
-      Pr, \<Delta> \<turnstile> \<langle>e; \<omega>\<rangle> [\<Down>]\<^sub>t Val (VBool True); 
+      Pr, \<Delta> \<turnstile> \<langle>e; \<omega>\<rangle> [\<Down>]\<^sub>t (Val (VBool True)); 
       red_inhale Pr \<Delta> havoc_new A \<omega> res \<rbrakk> \<Longrightarrow>
       red_inhale Pr \<Delta> havoc_new (Imp e A) \<omega> res" 
  | InhImpFalse:  
@@ -232,14 +54,14 @@ inductive red_inhale :: "program \<Rightarrow> 'a interp \<Rightarrow> bool \<Ri
        wd_pure_exp_total Pr \<Delta> CInhale e_r \<omega>;
        wd_pure_exp_total Pr \<Delta> CInhale e_p \<omega>;
        \<omega>' \<in> inhale_perm_single havoc_new \<omega> (a,f) (Some (Abs_prat p))\<rbrakk> \<Longrightarrow>
-       red_inhale Pr \<Delta> havoc_new (Atomic (Acc e_r f e_p)) \<omega> (RNormal \<omega>')"
+       red_inhale Pr \<Delta> havoc_new (Atomic (Acc e_r f (PureExp e_p))) \<omega> (RNormal \<omega>')"
  | InhAssumeAccFail1: 
     "\<lbrakk> Pr, \<Delta> \<turnstile> \<langle>e_r; \<omega>\<rangle> [\<Down>]\<^sub>t Val (VRef Null) \<rbrakk> \<Longrightarrow> 
-      red_inhale Pr \<Delta> havoc_new (Atomic (Acc e_r f e_p)) \<omega> RMagic"
+      red_inhale Pr \<Delta> havoc_new (Atomic (Acc e_r f (PureExp e_p))) \<omega> RMagic"
  | InhAssumeAccFail2: 
     "\<lbrakk> Pr, \<Delta> \<turnstile> \<langle>e_r; \<omega>\<rangle> [\<Down>]\<^sub>t Val (VRef (Address a)); Pr, \<Delta> \<turnstile> \<langle>e_p; \<omega>\<rangle> [\<Down>]\<^sub>t Val (VPerm p); 
       (\<not>wd_pure_exp_total Pr \<Delta> CInhale e_r \<omega> \<or> \<not>wd_pure_exp_total Pr \<Delta> CInhale e_r \<omega> \<or> p < 0)\<rbrakk> \<Longrightarrow>
-      red_inhale Pr \<Delta> havoc_new (Atomic (Acc e_r f e_p)) \<omega> RFailure"
+      red_inhale Pr \<Delta> havoc_new (Atomic (Acc e_r f (PureExp e_p))) \<omega> RFailure"
 (** inhale/assume acc(e.f, wildcard) **)
 (*  \<omega>' \<in> plus_total_full_set {\<omega>} 
         singleton_total_wildcard havoc_new (r,f) (get_heap_total_full \<omega> (r,f)) (get_store_total \<omega>) (get_trace_total \<omega>)) *)
@@ -247,15 +69,15 @@ inductive red_inhale :: "program \<Rightarrow> 'a interp \<Rightarrow> bool \<Ri
     "\<lbrakk> Pr, \<Delta> \<turnstile> \<langle>e_r; \<omega>\<rangle> [\<Down>]\<^sub>t Val (VRef (Address a));
        (wd_pure_exp_total Pr \<Delta> CInhale e_r \<omega>);
        \<omega>' \<in> inhale_perm_single havoc_new \<omega> (a,f) None \<rbrakk> \<Longrightarrow>
-       red_inhale Pr \<Delta> havoc_new (Atomic (AccWildcard e_r f)) \<omega> (RNormal \<omega>')"
+       red_inhale Pr \<Delta> havoc_new (Atomic (Acc e_r f Wildcard)) \<omega> (RNormal \<omega>')"
   | InhAssumeAccWildcardFail1: 
     "\<lbrakk> Pr, \<Delta> \<turnstile> \<langle>e_r; \<omega>\<rangle> [\<Down>]\<^sub>t Val (VRef Null) \<rbrakk> \<Longrightarrow> 
-    red_inhale Pr \<Delta> havoc_new (Atomic (AccWildcard e_r f)) \<omega> RMagic"
+    red_inhale Pr \<Delta> havoc_new (Atomic (Acc e_r f Wildcard)) \<omega> RMagic"
  | InhAssumeAccWildcardFail2: 
      "\<lbrakk> Pr, \<Delta> \<turnstile> \<langle>e_r; \<omega>\<rangle> [\<Down>]\<^sub>t Val (VRef (Address a)); 
         Pr, \<Delta> \<turnstile> \<langle>e_p; \<omega>\<rangle> [\<Down>]\<^sub>t Val (VPerm p); 
        \<not>wd_pure_exp_total Pr \<Delta> CInhale e_r \<omega>\<rbrakk> \<Longrightarrow>
-    red_inhale Pr \<Delta> havoc_new (Atomic (AccWildcard e_r f)) \<omega> RFailure"
+    red_inhale Pr \<Delta> havoc_new (Atomic (Acc e_r f Wildcard)) \<omega> RFailure"
 (** others **)
  | InhInhaleExhale: 
     "\<lbrakk> red_inhale Pr \<Delta> havoc_new A \<omega> res \<rbrakk> \<Longrightarrow> 
@@ -318,11 +140,11 @@ inductive red_exhale :: "program \<Rightarrow> 'a interp \<Rightarrow> 'a full_t
        wd_pure_exp_total Pr \<Delta> (CExhale locs) e_r \<omega>;
        wd_pure_exp_total Pr \<Delta> (CExhale locs) e_p \<omega>;
        m' = m( (a,f) := Abs_prat ( (Rep_prat (m((a, f)))) - p) ) \<rbrakk> \<Longrightarrow>
-       red_exhale Pr \<Delta> \<omega>0 (Atomic (Acc e_r f e_p)) m (ExhaleNormal m')"
+       red_exhale Pr \<Delta> \<omega>0 (Atomic (Acc e_r f (PureExp e_p))) m (ExhaleNormal m')"
   | ExhAccFail1: 
     "\<lbrakk> Pr, \<Delta> \<turnstile> \<langle>e_r; \<omega>\<rangle> [\<Down>]\<^sub>t Val (VRef r); Pr, \<Delta> \<turnstile> \<langle>e_p; \<omega>\<rangle> [\<Down>]\<^sub>t Val (VPerm p); 
       (r = Null \<or> \<not>wd_pure_exp_total Pr \<Delta> (CExhale locs) e_r \<omega> \<or> \<not>wd_pure_exp_total Pr \<Delta> (CExhale locs) e_p \<omega> \<or> p < 0)\<rbrakk> \<Longrightarrow>
-      red_exhale Pr \<Delta> \<omega>0 (Atomic (Acc e_r f e_p)) m ExhaleFailure"
+      red_exhale Pr \<Delta> \<omega>0 (Atomic (Acc e_r f (PureExp e_p))) m ExhaleFailure"
   | ExhAccFail2:
     "\<lbrakk> \<omega> = update_mask_total_full \<omega>0 m;
        Pr, \<Delta> \<turnstile> \<langle>e_r; \<omega>\<rangle> [\<Down>]\<^sub>t Val (VRef (Address a));
@@ -331,7 +153,7 @@ inductive red_exhale :: "program \<Rightarrow> 'a interp \<Rightarrow> 'a full_t
        wd_pure_exp_total Pr \<Delta> (CExhale locs) e_p \<omega>;
        p \<ge> 0; 
        \<not> (pgte (m(a,f)) (Abs_prat p)) \<rbrakk> \<Longrightarrow>
-       red_exhale Pr \<Delta> \<omega>0 (Atomic (Acc e_r f e_p)) m ExhaleFailure"
+       red_exhale Pr \<Delta> \<omega>0 (Atomic (Acc e_r f (PureExp e_p))) m ExhaleFailure"
 
 \<comment>\<open>exhale acc(e.f, wildcard)\<close>
  \<comment>\<open>Exhaling wildcard removes some non-zero permission this is less than the current permission held\<close>
@@ -342,17 +164,17 @@ inductive red_exhale :: "program \<Rightarrow> 'a interp \<Rightarrow> 'a full_t
        pgt (m(a,f)) (Abs_prat p);
        wd_pure_exp_total Pr \<Delta> (CExhale locs) e_r \<omega>;
        m' = m( (a,f) := Abs_prat ( (Rep_prat (m((a, f)))) - p) ) \<rbrakk> \<Longrightarrow>
-       red_exhale Pr \<Delta> \<omega>0 (Atomic (AccWildcard e_r f)) m (ExhaleNormal m')"
+       red_exhale Pr \<Delta> \<omega>0 (Atomic (Acc e_r f Wildcard)) m (ExhaleNormal m')"
   | ExhAccWildcardFail1:
     "\<lbrakk> Pr, \<Delta> \<turnstile> \<langle>e_r; \<omega>\<rangle> [\<Down>]\<^sub>t Val (VRef r); 
       (r = Null \<or> \<not>wd_pure_exp_total Pr \<Delta> (CExhale locs) e_r \<omega>)\<rbrakk> \<Longrightarrow>
-      red_exhale Pr \<Delta> \<omega>0 (Atomic (AccWildcard e_r f)) m ExhaleFailure"
+      red_exhale Pr \<Delta> \<omega>0 (Atomic (Acc e_r f Wildcard)) m ExhaleFailure"
   | ExhAccWildcardFail2:
     "\<lbrakk> \<omega> = update_mask_total_full \<omega>0 m;
        Pr, \<Delta> \<turnstile> \<langle>e_r; \<omega>\<rangle> [\<Down>]\<^sub>t Val (VRef (Address a));
        wd_pure_exp_total Pr \<Delta> (CExhale locs) e_r \<omega>;
        (m(a,f)) = pnone \<rbrakk> \<Longrightarrow>
-      red_exhale Pr \<Delta> \<omega>0 (Atomic (AccWildcard e_r f)) m ExhaleFailure"
+      red_exhale Pr \<Delta> \<omega>0 (Atomic (Acc e_r f Wildcard)) m ExhaleFailure"
  
 \<comment>\<open>exhale other cases\<close>
   | ExhInhaleExhale: 
