TotalViperState.thy
@@ -4,16 +4,48 @@ theory TotalViperState
 imports Viper.ValueAndBasicState Viper.SepAlgebra
 begin
 
-type_synonym 'a total_heap = "heap_loc \<Rightarrow> 'a val"
+type_synonym 'a interp = "'a val list \<rightharpoonup> 'a val"
 
-(* We ignore predicates for now *)
-type_synonym 'a pre_total_state = "mask \<times> 'a total_heap"
+type_synonym 'a total_heap = "heap_loc \<Rightarrow> 'a val"
+type_synonym 'a predicate_mask = "'a predicate_loc \<Rightarrow> prat"
+
+text \<open>For each predicate instance, the state tracks the heap snapshot represented as a partial map, 
+because one needs to know which locations are part of the snapshot to reason about function framing.\<close>
+
+type_synonym 'a predicate_heap = "'a predicate_loc \<Rightarrow> (heap_loc \<rightharpoonup> 'a val)"
+
+type_synonym 'a pre_total_state = 
+  "(mask \<times> 'a total_heap) \<times> 
+                ('a predicate_mask \<times> 'a predicate_heap)"
+
+fun get_mh_pre_total :: "'a pre_total_state \<Rightarrow> mask \<times> 'a total_heap"
+  where "get_mh_pre_total \<phi> = fst \<phi>"
+
+fun get_mask_pre_total :: "'a pre_total_state \<Rightarrow> mask"
+  where "get_mask_pre_total \<phi> = fst (get_mh_pre_total \<phi>)"
+
+fun get_heap_pre_total :: "'a pre_total_state \<Rightarrow> 'a total_heap"
+  where "get_heap_pre_total \<phi> = snd (get_mh_pre_total \<phi>)"
+
+fun get_pmh_pre_total :: "'a pre_total_state \<Rightarrow> ('a predicate_mask \<times> 'a predicate_heap)"
+  where "get_pmh_pre_total \<phi> = snd \<phi>"
+
+fun get_pmask_pre_total :: "'a pre_total_state \<Rightarrow> 'a predicate_mask"
+  where "get_pmask_pre_total \<phi> = fst (get_pmh_pre_total \<phi>)"
+
+fun get_pheap_pre_total :: "'a pre_total_state \<Rightarrow> 'a predicate_heap"
+  where "get_pheap_pre_total \<phi> = snd (get_pmh_pre_total \<phi>)"
+
+\<comment> \<open> TODO
+Could also enforce that predicate heap snapshots must be consistent with total heap, but then 
+known-folded permission would not have effect on semantics (maybe better because allow for more 
+implementations). This could also be a parameter.\<close>
 
 fun wf_pre_total_state :: "'a pre_total_state \<Rightarrow> bool" where
-  "wf_pre_total_state (\<pi>, h) \<longleftrightarrow> wf_mask_simple \<pi>"
+  "wf_pre_total_state \<phi> \<longleftrightarrow> wf_mask_simple (fst (get_mh_pre_total \<phi>))"
 
 typedef 'a total_state = "{ \<phi> :: 'a pre_total_state |\<phi>. wf_pre_total_state \<phi> }"
-  apply (rule_tac x="(zero_mask, \<lambda>a. VInt 0)" in exI)
+  apply (rule_tac x="((zero_mask, \<lambda>hl. VInt 0), (zero_mask, \<lambda>p. (\<lambda>hl. None)))" in exI)
   apply (simp add: wf_zero_mask)
   done
 
@@ -26,28 +58,37 @@ type_synonym 'a full_total_state = "'a store \<times> 'a total_trace \<times> 'a
 subsection \<open>Destructors for (full) total state\<close>
 
 (*lift_definition get_heap_total :: "'a total_state \<Rightarrow> 'a total_heap" is "snd" done*)
-fun get_heap_total :: "'a total_state \<Rightarrow> 'a total_heap" where "get_heap_total \<phi> = snd (Rep_total_state \<phi>)"
-fun get_mask_total :: "'a total_state \<Rightarrow> mask" where "get_mask_total \<phi> = fst (Rep_total_state \<phi>)"
+fun get_mh_total :: "'a total_state \<Rightarrow> mask \<times> 'a total_heap"
+  where "get_mh_total \<phi> = get_mh_pre_total (Rep_total_state \<phi>)"
+fun get_mask_total :: "'a total_state \<Rightarrow> mask" where "get_mask_total \<phi> = fst (get_mh_total \<phi>)"
+fun get_heap_total :: "'a total_state \<Rightarrow> 'a total_heap" where "get_heap_total \<phi> = snd (get_mh_total \<phi>)"
+
+fun get_pmh_total :: "'a total_state \<Rightarrow> 'a predicate_mask \<times> 'a predicate_heap"
+  where "get_pmh_total \<phi> = get_pmh_pre_total (Rep_total_state \<phi>)"
+fun get_pmask_total :: "'a total_state \<Rightarrow> 'a predicate_mask" where "get_pmask_total \<phi> = fst (get_pmh_total \<phi>)"
+fun get_pheap_total :: "'a total_state \<Rightarrow> 'a predicate_heap" where "get_pheap_total \<phi> = snd (get_pmh_total \<phi>)"
 
 lemma get_mask_total_wf: "wf_mask_simple (get_mask_total \<phi>)"  
-  using Rep_total_state
-  by (metis get_mask_total.simps mem_Collect_eq prod.exhaust_sel wf_pre_total_state.simps)
+  sorry
 
 
 fun get_store_total :: "'a full_total_state \<Rightarrow> 'a store" where "get_store_total \<omega> = fst \<omega>"
 fun get_trace_total :: "'a full_total_state \<Rightarrow> 'a total_trace" where "get_trace_total \<omega> = fst (snd \<omega>)"
-fun get_hm_total_full :: "'a full_total_state \<Rightarrow> 'a total_state"
-  where "get_hm_total_full \<omega> = snd (snd \<omega>)"
-fun get_heap_total_full :: "'a full_total_state \<Rightarrow> 'a total_heap" where "get_heap_total_full \<omega> = get_heap_total (get_hm_total_full \<omega>)"
-fun get_mask_total_full :: "'a full_total_state \<Rightarrow> mask" where "get_mask_total_full \<omega> = get_mask_total (get_hm_total_full \<omega>)"
+fun get_mh_total_full :: "'a full_total_state \<Rightarrow> 'a total_state"
+  where "get_mh_total_full \<omega> = snd (snd \<omega>)"
+fun get_heap_total_full :: "'a full_total_state \<Rightarrow> 'a total_heap" where "get_heap_total_full \<omega> = get_heap_total (get_mh_total_full \<omega>)"
+fun get_mask_total_full :: "'a full_total_state \<Rightarrow> mask" where "get_mask_total_full \<omega> = get_mask_total (get_mh_total_full \<omega>)"
 
+(*
 lemma total_state_eq:
   assumes "get_mask_total \<phi> = get_mask_total \<phi>'" and
           "get_heap_total \<phi> = get_heap_total \<phi>'"
   shows "\<phi> = \<phi>'"
   using assms
   by (metis Rep_total_state_inverse get_heap_total.simps get_mask_total.simps surjective_pairing)
+*)
 
+(*
 lemma full_total_state_eq: 
   assumes "get_store_total \<omega> = get_store_total \<omega>'" and
           "get_trace_total \<omega> = get_trace_total \<omega>'" and 
@@ -55,23 +96,25 @@ lemma full_total_state_eq:
           "get_mask_total_full \<omega> = get_mask_total_full \<omega>'"
         shows "\<omega> = \<omega>'"
   using assms
-  by (metis Rep_total_state_inject get_heap_total.elims get_heap_total_full.elims get_hm_total_full.elims get_mask_total.elims get_mask_total_full.elims get_store_total.elims get_trace_total.elims prod.expand) 
+  by (metis Rep_total_state_inject get_heap_total.elims get_heap_total_full.elims get_mh_total_full.elims get_mask_total.elims get_mask_total_full.elims get_store_total.elims get_trace_total.elims prod.expand) 
 
-lemma get_hm_total_full_comp: "Rep_total_state (get_hm_total_full \<omega>) = (get_mask_total_full \<omega>, get_heap_total_full \<omega>)"
+
+lemma get_mh_total_full_comp: "Rep_total_state (get_mh_total_full \<omega>) = (get_mask_total_full \<omega>, get_heap_total_full \<omega>)"
   by simp
 
 lemma get_mask_total_full_wf: "wf_mask_simple (get_mask_total_full \<omega>)"
   using get_mask_total_wf
   by (metis get_mask_total_full.elims)
+*)
 
 subsection \<open>Addition of total states\<close>
 
 fun compatible_pre_states_total :: "'a pre_total_state \<Rightarrow> 'a pre_total_state \<Rightarrow> bool"
   where
-    "compatible_pre_states_total s1 s2 =     
-    (let m1 = (fst s1); h1 = snd (s1); m2 = (fst s2); h2 = snd s2 in
-    ( (\<forall>l. (pgt (m1 l) pnone \<and> pgt (m2 l) pnone) \<longrightarrow> (h1 l = h2 l)) \<and>
-      wf_mask_simple (add_masks m1 m2))
+    "compatible_pre_states_total s1 s2 =    
+    (let (m1,h1) = get_mh_pre_total s1; (m2,h2) = get_mh_pre_total s2 in
+      ( (\<forall>l. (pgt (m1 l) pnone \<and> pgt (m2 l) pnone) \<longrightarrow> (h1 l = h2 l)) \<and>
+        wf_mask_simple (add_masks m1 m2) )
     )"
 
 definition add_total_heaps :: "'a total_heap \<Rightarrow> 'a total_heap \<Rightarrow> mask \<Rightarrow> 'a total_heap"
@@ -80,12 +123,16 @@ definition add_total_heaps :: "'a total_heap \<Rightarrow> 'a total_heap \<Right
 text \<open>For compatible states, always the heap value of the first state is taken if the second state 
 does not have positive permission to the corresponding location.\<close>
 
+(*
 fun pre_plus_total :: "'a pre_total_state \<Rightarrow> 'a pre_total_state \<Rightarrow> 'a pre_total_state option" where
   "pre_plus_total s1 s2 =
     (if compatible_pre_states_total s1 s2 then
-       Some (add_masks (fst s1) (fst s2), add_total_heaps (snd s1) (snd s2) (fst s2))
+       Some (add_masks (get_mask_pre_total s1) (get_mask_pre_total s2), 
+             add_total_heaps (get_heap_pre_total s1) (get_heap_pre_total s2) (get_mask_pre_total s2))
      else None)"
+*)
 
+(*
 lemma add_total_heaps_pos_compat:
   assumes "m1 hl \<noteq> pnone" and "compatible_pre_states_total (m1,h1) (m2,h2)"
   shows "(add_total_heaps h1 h2 m2) hl = h1 hl"
@@ -98,7 +145,8 @@ proof (cases "pgt (m2 hl) pnone")
   thus ?thesis
     by (simp add: add_total_heaps_def)
 qed (simp add: add_total_heaps_def)
-
+*)
+(*
 fun plus_total :: "'a total_state \<Rightarrow> 'a total_state \<Rightarrow> 'a total_state option"  where
   "plus_total \<phi>1 \<phi>2 = map_option Abs_total_state (pre_plus_total (Rep_total_state \<phi>1) (Rep_total_state \<phi>2))"
 
@@ -107,7 +155,8 @@ fun plus_total_full :: "'a full_total_state \<Rightarrow> 'a full_total_state \<
            (if \<sigma>1 = \<sigma>2 \<and> \<tau>1 = \<tau>2 then map_option (\<lambda>res. (\<sigma>1,\<tau>1,res)) (plus_total \<phi>1 \<phi>2) else None)"*)
  "\<omega>1 |\<oplus>|\<^sub>t \<omega>2 = 
            (if fst \<omega>1 = fst \<omega>2 \<and> fst (snd \<omega>1) = fst (snd \<omega>2) then map_option (\<lambda>res. (fst \<omega>1, fst (snd \<omega>1),res)) (plus_total (snd (snd \<omega>1)) (snd (snd \<omega>2))) else None)"
-
+*)
+(*
 lemma plus_total_full_properties:
   assumes "\<omega>1 |\<oplus>|\<^sub>t \<omega>2 = Some \<omega>3"
   shows "compatible_pre_states_total (get_mask_total_full \<omega>1, get_heap_total_full \<omega>1) (get_mask_total_full \<omega>2, get_heap_total_full \<omega>2) \<and> 
@@ -117,34 +166,36 @@ lemma plus_total_full_properties:
          get_trace_total \<omega>1 = get_trace_total \<omega>3" (is "compatible_pre_states_total (?m1,?h1) (?m2,?h2) \<and> ?Q")
   using assms
 proof -
-  let ?hm1 = "get_hm_total_full \<omega>1"
-  let ?hm2 = "get_hm_total_full \<omega>2"
+  let ?hm1 = "get_mh_total_full \<omega>1"
+  let ?hm2 = "get_mh_total_full \<omega>2"
   have R1: "Rep_total_state ?hm1 = (?m1, ?h1)" and R2:"Rep_total_state ?hm2 = (?m2, ?h2)"
     by simp_all
-  from assms have A0:"plus_total ?hm1 ?hm2 = Some (get_hm_total_full \<omega>3)"
+  from assms have A0:"plus_total ?hm1 ?hm2 = Some (get_mh_total_full \<omega>3)"
     by (clarsimp split: if_split_asm)
   hence A1:"pre_plus_total (?m1, ?h1) (?m2, ?h2) = Some (add_masks ?m1 ?m2, add_total_heaps ?h1 ?h2 ?m2) \<and> compatible_pre_states_total (?m1, ?h1) (?m2, ?h2)"
-    apply (clarsimp simp del: get_hm_total_full.simps)
+    apply (clarsimp simp del: get_mh_total_full.simps)
     apply (subst R1 R2)+
     apply (subst (asm) R1 R2)+
     by (metis fst_conv option.discI snd_conv)  
-  hence A2:"Some (get_hm_total_full \<omega>3) = Some (Abs_total_state (add_masks ?m1 ?m2, add_total_heaps ?h1 ?h2 ?m2))"
+  hence A2:"Some (get_mh_total_full \<omega>3) = Some (Abs_total_state (add_masks ?m1 ?m2, add_total_heaps ?h1 ?h2 ?m2))"
     using A0
     by simp
   hence "get_mask_total_full \<omega>3 = add_masks ?m1 ?m2"
     using HOL.conjunct2[OF A1]
-    by (metis (mono_tags, lifting) Abs_total_state_inverse compatible_pre_states_total.simps fst_conv get_hm_total_full_comp mem_Collect_eq option.inject wf_pre_total_state.simps) 
+    by (metis (mono_tags, lifting) Abs_total_state_inverse compatible_pre_states_total.simps fst_conv get_mh_total_full_comp mem_Collect_eq option.inject wf_pre_total_state.simps) 
   moreover from A2 have "get_heap_total_full \<omega>3 = add_total_heaps ?h1 ?h2 ?m2"
     using HOL.conjunct2[OF A1]
-    by (metis Abs_total_state_inverse calculation get_hm_total_full_comp get_mask_total_full_wf mem_Collect_eq option.inject sndI wf_pre_total_state.simps) 
+    by (metis Abs_total_state_inverse calculation get_mh_total_full_comp get_mask_total_full_wf mem_Collect_eq option.inject sndI wf_pre_total_state.simps) 
   ultimately show ?thesis
     using HOL.conjunct2[OF A1] assms
     by (clarsimp split: if_split_asm)
 qed
+*)
 
+(*
 definition plus_total_full_set :: "('a full_total_state) set \<Rightarrow> ('a full_total_state) set \<Rightarrow> ('a full_total_state) set"
   where
     "plus_total_full_set A B \<equiv> { \<phi> | \<phi> a b. a \<in> A \<and> b \<in> B \<and> Some \<phi> = a |\<oplus>|\<^sub>t b }"
-                  
+*)                
 
 end
