TotalUtil.thy
@@ -1,0 +1,153 @@
+theory TotalUtil
+imports Viper.ViperLang Viper.ValueAndBasicState TotalViperState
+begin
+
+fun update_store_total :: "'a full_total_state \<Rightarrow> var \<Rightarrow> 'a val \<Rightarrow> 'a full_total_state"
+  where "update_store_total \<omega> x v = ((get_store_total \<omega>)(x \<mapsto> v), get_trace_total \<omega>, get_mh_total_full \<omega>)"
+
+lemma update_store_total_trace_same: "get_trace_total (update_store_total \<omega> x v) = get_trace_total \<omega>"
+  by simp
+
+lemma update_store_total_hm_same: "get_mh_total_full (update_store_total \<omega> x v) = get_mh_total_full \<omega>"
+  by simp
+
+lemma update_store_total_heap_same: "get_heap_total_full (update_store_total \<omega> x v) = get_heap_total_full \<omega>"
+  by simp
+
+lemma update_store_total_mask_same: "get_mask_total_full (update_store_total \<omega> x v) = get_mask_total_full \<omega>"
+  by simp
+
+fun update_trace_total :: "'a full_total_state \<Rightarrow> 'a total_trace \<Rightarrow> 'a full_total_state"
+  where "update_trace_total \<omega> \<pi> = (get_store_total \<omega>, \<pi>, get_mh_total_full \<omega>)"
+
+lemma update_trace_total_store_same: "get_store_total (update_trace_total \<omega> \<pi>) = get_store_total \<omega>"
+  by simp
+
+lemma update_trace_total_hm_same: "get_mh_total_full (update_trace_total \<omega> \<pi>) = get_mh_total_full \<omega>"
+  by simp
+
+lemma update_trace_total_heap_same: "get_heap_total_full (update_trace_total \<omega> \<pi>) = get_heap_total_full \<omega>"
+  by simp
+
+lemma update_trace_total_mask_same: "get_mask_total_full (update_trace_total \<omega> \<pi>) = get_mask_total_full \<omega>"
+  by simp
+
+definition update_heap_total :: "'a total_state \<Rightarrow> heap_loc \<Rightarrow> 'a val \<Rightarrow> 'a total_state"
+  where "update_heap_total \<phi> l v = Abs_total_state ( ((get_mask_total \<phi>), (get_heap_total \<phi>)(l := v)), get_pmh_total \<phi>)"
+
+definition update_mask_total :: "'a total_state \<Rightarrow> mask \<Rightarrow> 'a total_state"
+  where "update_mask_total \<phi> m' = Abs_total_state ((m', get_heap_total \<phi>), get_pmh_total \<phi>)"
+
+lemma Abs_total_state_inverse_2:
+  assumes "wf_pre_total_state (m,h)"
+  shows "Rep_total_state (Abs_total_state (m,h)) = (m,h)"
+  using assms Abs_total_state_inverse
+  by blast
+
+lemma get_update_mask_total: 
+  assumes "wf_mask_simple m0"
+  shows   "get_mask_total (update_mask_total mh m0) = m0"
+  unfolding update_mask_total_def
+  using assms
+  by (simp add: Abs_total_state_inverse_2)
+
+lemma update_mask_total_multiple: 
+  assumes "wf_mask_simple m0" and "wf_mask_simple m2"
+  shows   "update_mask_total (update_mask_total mh m0) m1 = update_mask_total mh m1"
+  unfolding update_mask_total_def  
+  using assms
+  by (simp add: Abs_total_state_inverse_2)
+
+lemma update_heap_total_mask_same: "get_mask_total (update_heap_total \<phi> l v) = get_mask_total \<phi>"
+  unfolding update_heap_total_def
+  (*
+  by (metis Abs_total_state_inverse_2 fst_conv get_mask_total.simps get_mask_total_wf wf_pre_total_state.simps)*)
+  sorry
+
+lemma Rep_total_state_inj: "Rep_total_state a = Rep_total_state b \<Longrightarrow> a = b"
+  by (metis Rep_total_state_inverse)
+
+lemma update_heap_total_overwrite: "update_heap_total (update_heap_total mh l v1) l v2 = update_heap_total mh l v2"
+ (* apply (rule total_state_eq)
+   apply (simp only: update_heap_total_mask_same)
+  by (metis Abs_total_state_inverse_2 fun_upd_upd get_heap_total.simps get_mask_total_wf snd_conv update_heap_total_def wf_pre_total_state.simps)*)
+  sorry
+
+lemma update_heap_total_lookup_1: "get_heap_total (update_heap_total \<phi> l v) l = v"
+ (* by (metis (no_types, lifting) Abs_total_state_inverse_2 fun_upd_eqD fun_upd_triv get_heap_total.simps get_mask_total_wf snd_conv update_heap_total_def wf_pre_total_state.simps) *)
+  sorry
+
+lemma update_heap_total_lookup_2: "l1 \<noteq> l2 \<Longrightarrow> get_heap_total (update_heap_total \<phi> l1 v) l2 = get_heap_total \<phi> l2"
+(*  by (metis (no_types, lifting) Abs_total_state_inverse_2 fun_upd_idem_iff fun_upd_triv fun_upd_twist get_heap_total.elims get_mask_total_wf sndI update_heap_total_def wf_pre_total_state.simps) *)
+  sorry
+
+fun update_heap_total_full :: "'a full_total_state \<Rightarrow> heap_loc \<Rightarrow> 'a val \<Rightarrow> 'a full_total_state"
+  where "update_heap_total_full \<omega> l v = (get_store_total \<omega>, get_trace_total \<omega>, update_heap_total (get_mh_total_full \<omega>) l v )"
+
+lemma update_heap_total_full_lookup_1: "get_heap_total_full (update_heap_total_full \<phi> l v) l = v"
+  by (metis get_heap_total_full.simps get_mh_total_full.simps snd_conv update_heap_total_full.simps update_heap_total_lookup_1)
+
+lemma update_heap_total_full_lookup_2: "l1 \<noteq> l2 \<Longrightarrow> get_heap_total_full (update_heap_total_full \<phi> l1 v) l2 = get_heap_total_full \<phi> l2"
+  by (metis get_heap_total_full.simps get_mh_total_full.simps snd_conv update_heap_total_full.simps update_heap_total_lookup_2)
+
+lemma update_heap_total_overwrite_full: "update_heap_total_full (update_heap_total_full \<omega> l v1) l v2 = update_heap_total_full \<omega> l v2"
+  sorry
+ (* apply (rule full_total_state_eq)
+     apply simp
+    apply simp
+   apply (simp add: update_heap_total_overwrite)
+  by (metis get_mh_total_full.elims get_mask_total_full.elims snd_conv update_heap_total_full.simps update_heap_total_mask_same)*)
+  
+fun update_mask_total_full :: "'a full_total_state \<Rightarrow> mask \<Rightarrow> 'a full_total_state"
+  where "update_mask_total_full \<omega> m = (get_store_total \<omega>, get_trace_total \<omega>, update_mask_total (get_mh_total_full \<omega>) m)"
+
+lemma update_heap_total_full_mask_same: "get_mask_total_full (update_heap_total_full \<omega> l v) = get_mask_total_full \<omega>"
+  by (metis get_mh_total_full.simps get_mask_total_full.simps snd_conv update_heap_total_full.simps update_heap_total_mask_same)
+
+lemma get_update_mask_total_full: 
+  assumes "wf_mask_simple m0"
+  shows   "get_mask_total_full (update_mask_total_full mh m0) = m0"
+  using assms get_update_mask_total
+  by auto
+
+lemma update_mask_total_full_same:
+  "(update_mask_total_full \<omega> (get_mask_total_full \<omega>)) = \<omega>"
+  by (simp add: update_mask_total_def Rep_total_state_inverse)
+
+lemma update_mask_total_same_heap: 
+  assumes "wf_mask_simple m"
+  shows "get_heap_total (update_mask_total \<phi> m) = get_heap_total \<phi>"
+  unfolding update_mask_total_def
+  using assms
+  by (simp add: Abs_total_state_inverse)
+
+lemma update_mask_total_full_same_heap: 
+  assumes "wf_mask_simple m"
+  shows "get_heap_total_full (update_mask_total_full \<phi> m) = get_heap_total_full \<phi>"
+  using assms update_mask_total_same_heap
+  by auto
+  
+lemma update_mask_total_full_multiple: 
+  assumes "wf_mask_simple m0"
+  shows   "update_mask_total_full (update_mask_total_full \<omega> m0) m1 = update_mask_total_full \<omega> m1"
+  using assms
+  using update_mask_total_multiple by fastforce
+
+
+fun map_result_2 :: "(mask \<Rightarrow> (mask set) option) \<Rightarrow> (mask set) option \<Rightarrow> (mask set) option"
+  where 
+    "map_result_2 f None = None"
+  | "map_result_2 f (Some xs) = (if \<exists>x \<in> xs. f x = None then None else Some (\<Union>x \<in> xs. the (f x))) "
+
+
+fun get_address_opt :: "'a val \<Rightarrow> address option"
+  where 
+    "get_address_opt (VRef (Address a)) = Some a"
+  | "get_address_opt _ = None"
+
+fun option_fold :: "('a \<Rightarrow> 'b) \<Rightarrow> 'b \<Rightarrow> 'a option \<Rightarrow> 'b"
+  where 
+    "option_fold f e (Some x) = f x"
+  | "option_fold f e None = e"
+
+end
